finishing up

steel/apps/kvstore/Zeta.KeyValueStore.StateMachine.fst
@@ -5,10 +5,9 @@ module I = Zeta.Interleave
 
 module F = Zeta.KeyValueStore.Formats
 
-
-type log_entry =
-  | Vget: k:F.key_t -> v:F.value_t -> log_entry
-  | Vput: k:F.key_t -> v:F.value_t -> log_entry
+//
+// State of a key value store is a map from keys to optional values
+//
 
 type state = Map.t F.key_t (option F.value_t)
 
@@ -18,9 +17,26 @@ let get (st:state) (k:F.key_t) : option F.value_t =
 let put (st:state) (k:F.key_t) (v:F.value_t) : state =
   Map.upd st k (Some v)
 
-let initial_state : state = Map.const_on Set.empty None
+let initial_state : state = Map.const None
 
-let simulate_step (entry:log_entry) (st:state) : option state =
+//
+// Log entry is an operation on the state,
+//   either a get, or a put
+//
+
+type log_entry =
+  | Vget: k:F.key_t -> v:F.value_t -> log_entry
+  | Vput: k:F.key_t -> v:F.value_t -> log_entry
+
+type log = Seq.seq log_entry
+
+//
+// A single step of a state machine
+//
+// Returns None if the operation fails
+//
+
+let step (entry:log_entry) (st:state) : option state =
   match entry with
   | Vget k v ->
     let st_v = get st k in
@@ -29,23 +45,53 @@ let simulate_step (entry:log_entry) (st:state) : option state =
          if v' = v then Some st else None
   | Vput k v -> Some (put st k v)
 
-let rec simulate (s:Seq.seq log_entry)
+//
+// Sequence of steps
+//
+
+let rec steps (s:log)
   : Tot (option state)
         (decreases Seq.length s)
   = if Seq.length s = 0
     then Some initial_state
     else let s_pfx = SeqAux.prefix s (Seq.length s - 1) in
-         match simulate s_pfx with
+         match steps s_pfx with
          | None -> None
-         | Some st -> simulate_step (Seq.last s) st
+         | Some st -> step (Seq.last s) st
 
-type log = Seq.seq log_entry
 
-let valid_log (s:log) = Some? (simulate s)
+//
+// A log is valid if stepping through it succeeds
+//
+
+let valid_log (s:log) = Some? (steps s)
+
+//
+// Logs for multiple threads
+//
 
 type llog = Seq.seq log
 
+
+//
+// Definition of sequential consistency
+//
+
 let seq_consistent (ss:llog) = exists s. I.interleave s ss /\ valid_log s
+
+//
+// We prove sequential consistency,
+//   via a construction that's generic in the application functions
+//
+// The definition of sequential consistency for the generic construction
+//   is AppSimulate.seq_consistent
+//
+// Below, we prove that the generic definition can be specialized to
+//   the definition for key value store
+//
+// We sketch the statement of the lemma,
+//   then the rest of the module proves it
+//
 
 module AppSim = Zeta.AppSimulate
 module S = Zeta.KeyValueStore.Spec
@@ -59,45 +105,118 @@ let map_entry (e:app_log_entry) : log_entry =
   else let t : F.key_t & F.value_t = e.arg_cr in
        Vput (fst t) (snd t)
 
+let map_llog (ss:Seq.seq (Seq.seq app_log_entry)) : llog =
+  SeqAux.map (fun s -> SeqAux.map map_entry s) ss
+
+//
+// Following is the statement of the map lemma
+//
+
+val map_seq_consistency (ss:Seq.seq (Seq.seq app_log_entry))
+  : Lemma (requires AppSim.seq_consistent ss)
+          (ensures (seq_consistent (map_llog ss)))
+
+
+//
+// Rest of the module builds proof of map_seq_consistency
+//
+
+module App = Zeta.App
+module SA = Zeta.SeqAux
+
+//
+// Correspondence between the kv state and generic app state
+//
+
+let state_maps_app_state (st:state) (app_st:AppSim.app_state S.kv_params.adm) =
+  forall (k:F.key_t).
+    match Map.sel st k, app_st k with
+    | None, App.Null -> True
+    | Some v_st, App.DValue v_app_st -> v_st == v_app_st
+    | _, _ -> False
+
+let initial_state_maps_initial_app_state ()
+  : Lemma (state_maps_app_state initial_state (AppSim.init_app_state S.kv_params.adm))
+  = ()
+
+let map_fn_call (e:AppSim.appfn_call S.kv_params) : log_entry =
+  if e.fid_c = S.vget_id
+  then let t : F.key_t & F.value_t = e.arg_c in
+       Vget (fst t) (snd t)
+  else let t : F.key_t & F.value_t = e.arg_c in
+       Vput (fst t) (snd t)
+
+//
+// Simulating one step
+//
+
+let map_simulate_step
+  (fncall:AppSim.appfn_call S.kv_params)
+  (app_st:AppSim.app_state S.kv_params.adm)
+  (st:state)
+  : Lemma
+      (requires state_maps_app_state st app_st)
+      (ensures (let ropt = AppSim.simulate_step fncall app_st in
+                match ropt with
+                | None -> True  // under-specified
+                | Some (app_st, _res) ->
+                  let sopt = step (map_fn_call fncall) st in
+                  Some? sopt /\
+                  state_maps_app_state (Some?.v sopt) app_st))
+  = ()
+
+let prefix_map_lemma (#a #b:_) (s:Seq.seq a) (i:nat{i <= Seq.length s}) (f:a -> b)
+  : Lemma (SA.prefix (SA.map f s) i == SA.map f (SA.prefix s i))
+          [SMTPat (SA.prefix (SA.map f s) i)]
+  = assert (Seq.equal (SA.prefix (SA.map f s) i) (SA.map f (SA.prefix s i)))
+
+//
+// Simulating multiple steps
+//
+
+let rec map_simulate (fs:Seq.seq (AppSim.appfn_call S.kv_params))
+  : Lemma
+      (ensures (let ropt = AppSim.simulate fs in
+                match ropt with
+                | None -> True  // under-specified
+                | Some (app_st, _sres) ->
+                  let sopt = steps (SA.map map_fn_call fs) in
+                  Some? sopt /\
+                  state_maps_app_state (Some?.v sopt) app_st))
+      (decreases Seq.length fs)
+  = let n = Seq.length fs in
+    if n = 0
+    then ()
+    else begin
+      let fs_pfx = SA.prefix fs (n - 1) in
+      let sopt = AppSim.simulate fs_pfx in
+      map_simulate fs_pfx;
+      match sopt with
+      | None -> ()
+      | Some (app_st, _) ->
+        let Some st = steps (SA.map map_fn_call fs_pfx) in
+        map_simulate_step (Seq.index fs (n - 1)) app_st st
+    end
+
+let map_valid_call_result (is:Seq.seq app_log_entry)
+  : Lemma (requires AppSim.valid_call_result is)
+          (ensures valid_log (SA.map map_entry is))
+  = map_simulate (AppSim.app_fcs is);
+    assert (Seq.equal (SA.map map_entry is) (SA.map map_fn_call (AppSim.app_fcs is)))
+
 let map_log (s:Seq.seq app_log_entry) : log =
   SeqAux.map map_entry s
 
-let map_llog (ss:Seq.seq (Seq.seq app_log_entry)) : llog =
-  SeqAux.map map_log ss
-
-let map_interleaving (#n:nat) (il:I.interleaving app_log_entry n)
-  : I.interleaving log_entry n
-  = let open Zeta.Interleave in
-    SeqAux.map (fun i -> {
-      e = map_entry i.e;
-      s = i.s }) il
-
-let interleaving_iseq_commutes
-  (n:nat)
-  (s:Seq.seq app_log_entry)
-  (il:I.interleaving app_log_entry n)
-  : Lemma (requires I.i_seq il == s)
-          (ensures I.i_seq (map_interleaving il) == map_log s)
-  = let open Zeta.Interleave in
-    let aux (#a:_) (#n:_) (il:interleaving a n) (i:nat{i < Seq.length il})
-      : Lemma (ensures Seq.index (i_seq il) i == (Seq.index il i).e)
-              [SMTPat ()]
-      = I.lemma_iseq_index il i in
-    assert (Seq.equal (I.i_seq (map_interleaving il)) (map_log s))
-
-let interleaving_sseq_commutes
-  (n:nat)
-  (ss:Seq.seq (Seq.seq app_log_entry))
-  (il:I.interleaving app_log_entry n)
-  : Lemma (requires I.s_seq il == ss)
-          (ensures I.s_seq (map_interleaving il) == map_llog ss)
-  = admit ()
-
-let map_seq_consistency (ss:Seq.seq (Seq.seq (AppSim.appfn_call_res S.kv_params)))
+let map_seq_consistency (ss:Seq.seq (Seq.seq app_log_entry))
   : Lemma (requires AppSim.seq_consistent ss)
           (ensures (seq_consistent (map_llog ss)))
-  = eliminate exists is. I.interleave #(AppSim.appfn_call_res S.kv_params) is ss /\ AppSim.valid_call_result is
+  = eliminate exists (is:Seq.seq app_log_entry). I.interleave is ss /\ AppSim.valid_call_result is
     returns seq_consistent (map_llog ss)
     with _. begin
-      admit ()
+      I.map_interleave is ss map_entry;
+      assert (I.interleave (map_log is) (map_llog ss));
+      map_valid_call_result is;
+      introduce exists s. I.interleave s (map_llog ss) /\ valid_log s
+      with (map_log is)
+      and ()
     end
